Set svn:ignore propertly, extend language with labels

coq/playground/himp/domains.v
@@ -3,26 +3,56 @@ Require Import ZArith.
 Require Import FMapPositive.
 Require Import String.
 
+Require Import Setoid.
+
 Set Implicit Arguments.
 
-Axiom Map : Set -> Set.
-Axiom mapItem : forall {A: Set}, A -> Z -> Map A.
-Axiom mapJoin : forall {A : Set}, Map A -> Map A -> Map A.
-Axiom mapEmpty : forall {A : Set}, Map A.
+Inductive Map (Key Elt : Type) : Type :=
+| mapEmpty
+| mapItem (k : Key) (v : Elt)
+| mapJoin (m1 m2 : Map Key Elt)
+.
+Arguments mapEmpty [Key Elt].
+
 Infix ":->" := mapItem (at level 50, no associativity).
 Infix ":*" := mapJoin (at level 60, right associativity).
-Axiom mapUnit : forall {A} (m : Map A), m :* mapEmpty = m.
-Axiom mapComm : forall {A} (m1 m2 : Map A), m1 :* m2 = m2 :* m1.
-Axiom mapAssoc : forall {A} (m1 m2 m3 : Map A), (m1 :* m2) :* m3 = m1 :* m2 :* m3.
-Lemma mapComAssoc : forall {A} (m1 m2 m3 : Map A), m1 :* m2 :* m3 = m2 :* m1 :* m3.
-intros. rewrite <- mapAssoc, (mapComm m1 m2), mapAssoc. reflexivity.
-Qed.
+
+Inductive MapEquiv {K E : Type} : Map K E -> Map K E -> Prop :=
+| equivUnit : forall m, MapEquiv (m :* mapEmpty) m
+| equivComm : forall m1 m2, MapEquiv (m1 :* m2) (m2 :* m1)
+| equivAssoc : forall m1 m2 m3, MapEquiv ((m1 :* m2) :* m3) (m1 :* (m2 :* m3))
+
+| equivJoin : forall l1 r1 l2 r2, MapEquiv l1 l2 -> MapEquiv r1 r2 -> MapEquiv (l1 :* r1) (l2 :* r2)
+| equivTrans : forall m1 m2 m3, MapEquiv m1 m2 -> MapEquiv m2 m3 -> MapEquiv m1 m3
+| equivSym : forall m1 m2, MapEquiv m1 m2 -> MapEquiv m2 m1
+| equivRefl : forall m, MapEquiv m m
+.
+Infix "~=" := MapEquiv (at level 70, no associativity).
+
+Definition equivJoinL {K V} (r : Map K V) l1 l2 pfl : l1 :* r ~= l2 :* r :=
+  equivJoin pfl (equivRefl r).
+Definition equivJoinR {K V} (l : Map K V) r1 r2 pfr :  l :* r1 ~= l :* r2 :=
+  equivJoin (equivRefl l) pfr.
+
+Add Parametric Relation (K E : Type) : (Map K E) MapEquiv
+  reflexivity proved by equivRefl                        
+  symmetry proved by equivSym
+  transitivity proved by equivTrans
+  as map_equiv_rel.
+
+Add Parametric Morphism K E : (@mapJoin K E) with
+  signature MapEquiv ==> MapEquiv ==> MapEquiv as map_join_mor.
+Proof. auto using equivJoin. Qed.
+
+Lemma mapComAssoc : forall {K V} (m1 m2 m3 : Map K V), m1 :* m2 :* m3 ~= m2 :* m1 :* m3.
+intros. rewrite <- equivAssoc, (equivComm m1 m2), equivAssoc. reflexivity. Qed.
 
 (* Language syntax *)
 Inductive Exp :=
   | EVar (v:string)
   | ECon (i:Z)
   | EPlus (l r:Exp)
+  | EMinus (l r:Exp)
   | EDiv (l r:Exp)
   .
 Definition isEVal e :=
@@ -48,12 +78,16 @@ Inductive Stmt :=
   | Seq (s1 s2 : Stmt)
   | SIf (b:BExp) (sthn sels : Stmt)
   | SWhile (b:BExp) (body:Stmt)
+  | Jump (target : string)
   .
+
 
 (* K definitions *)
 Inductive freezer : Set :=
   | Fplusl : Exp -> freezer
   | Fplusr : Exp -> freezer
+  | Fminusl : Exp -> freezer
+  | Fminusr : Exp -> freezer
   | Fdivl : Exp -> freezer
   | Fdivr : Exp -> freezer
   | Flel : Exp -> freezer
@@ -71,10 +105,16 @@ Inductive kitem : Set :=
   | KBExp (b : BExp)
   | KStmt (s : Stmt)
   | KFreezer (f : freezer)
+  | KFreezeE (f : Exp -> kitem)
+  | KFreezeB (f : BExp -> kitem)
   .
 
 Definition kra : kitem -> list kitem -> list kitem := @cons kitem.
 Definition kdot : list kitem := nil.
 
-Inductive kcfg :=
-  | KCfg : list kitem -> Map string -> Map Z -> kcfg.
+Structure kcfg := KCfg {
+  kcell : list kitem;
+  store : Map string Z;
+  heap : Map Z Z;
+  labels : Map string Stmt
+  }.
